# 2.22

Let's consider the reduction of the following example:
```mermaid
(define (square-list items)
  (define (iter things answer)
    (if (null? things)
        answer
        (iter (cdr things)
              (cons (square (car things)) answer))))
  (iter items nil))
```

```
(square-list (list 1 2 3))
(1 . nill)
->
(4 . (1 . nill))
->
(9 . (4 . (1 . nill)))
->
(list 9 4 1)
```

So we recieve the reversed list because of order of cons params is wrong.
But.
We can't change order like in the following example:
```
(define (square-list items) (define (iter things answer)
    (if (null? things)
        answer
        (iter (cdr things)
              (cons answer
                    (square (car things))))))
  (iter items nil))
```

because nill shoulde be in the end of the list and we will recieve nill as the first elements:
```
(square-list (list 1 2 3))
(nill . 9)
->
((nill . 9) . 4)
->
(((nill . 9) . 4) . 1)
```

